ValueAnalysis (#221)
* Exploring: Add Sound.t inside ValueAnalysis

* Separate Unreach.v

* ValueAnalysis compiles with MLE

* Change Unreach.t from Prop to bool

This is for proving finiteness. We want to define a mapping function.
This may not be essential, but for comfort

* Add ge_nb in Unreach.t

* Add WF

* Revert "Add WF"

This reverts commit 50d7e9ec881b01957197b31a5d560cacec37f706.

* Add WF without changing type

* Strengthen unreach_compat

* Fix broken files

* Generalize Lineartyping

* Remove admits

Lprsv hle (#227)

* Add nb in Unreach.t

* WIP: add hle and simplifying VA

* WIP: tweaking; maybe rollback this

* Revert "WIP: tweaking; maybe rollback this"

This reverts commit 3ef8a7577a02763071f8e57e8166842e307f7c64.

* Redefine hle, WIP in VA.v

* Add nb_tac

* Housekeeping

* Housekeeping

* Housekeeping

* Housekeeping

* Housekeeping

Va strengthen (#248)

* Parameterize ValueAnalysis

* Relax ge of initial_mem_matches

* Rollback ge relaxation

backend/RTL.v
@@ -572,3 +572,11 @@ Proof.
   { apply X; auto. }
   unfold max_reg_function. xomega.
 Qed.
+
+Definition get_mem (st: state): mem :=
+  match st with
+  | State _ _ _ _ _ m0 => m0
+  | Callstate _ _ _ m0 => m0
+  | Returnstate _ _ m0 => m0
+  end
+.
