backend/Constpropproof.v
@@ -355,11 +355,11 @@ Ltac TransfInstr :=
 Lemma transf_step_correct:
   forall s1 t s2,
   step ge s1 t s2 ->
-  forall n1 s1' (SS: sound_state prog ge s1) (MS: match_states n1 s1 s1'),
+  forall n1 s1' (SS: exists su0, sound_state prog ge su0 s1) (MS: match_states n1 s1 s1'),
   (exists n2, exists s2', step tge s1' t s2' /\ match_states n2 s2 s2')
   \/ (exists n2, n2 < n1 /\ t = E0 /\ match_states n2 s2 s1')%nat.
 Proof.
-  induction 1; intros; inv MS; try InvSoundState; try (inv PC; try congruence).
+  induction 1; intros; inv MS; destruct SS as [su0 SS]; try InvSoundState; try (inv PC; try congruence).
 
 - (* Inop, preserved *)
   rename pc'0 into pc. TransfInstr; intros.
@@ -600,18 +600,20 @@ Qed.
 Theorem transf_program_correct:
   forward_simulation (RTL.semantics prog) (RTL.semantics tprog).
 Proof.
-  apply Forward_simulation with lt (fun n s1 s2 => sound_state prog ge s1 /\ match_states n s1 s2); constructor.
+  apply Forward_simulation with lt (fun n s1 s2 => (exists su0, sound_state prog ge su0 s1) /\ match_states n s1 s2); constructor.
 - apply lt_wf.
 - simpl; intros. exploit transf_initial_states; eauto. intros (n & st2 & A & B).
   exists n, st2; intuition. eapply sound_initial; eauto.
 - simpl; intros. destruct H. eapply transf_final_states; eauto.
 - simpl; intros. destruct H0.
-  assert (sound_state prog ge s1') by (eapply sound_step; eauto).
+  destruct H0 as [su0 SS].
+  assert (sound_state prog ge su0 s1') by (eapply sound_step; eauto).
   fold ge; fold tge.
   exploit transf_step_correct; eauto.
   intros [ [n2 [s2' [A B]]] | [n2 [A [B C]]]].
   exists n2; exists s2'; split; auto. left; apply plus_one; auto.
-  exists n2; exists s2; split; auto. right; split; auto. subst t; apply star_refl.
+  split; eauto.
+  exists n2; exists s2; split; eauto. right; split; auto. subst t; apply star_refl.
 - apply senv_preserved; auto.
 Qed.
 
