common/Unreach.v
@@ -1,0 +1,265 @@
+Require Import Coqlib Maps.
+Require Import AST Linking.
+Require Import Values Memory Globalenvs Events.
+Require Import RelationClasses.
+Require Import sflib.
+
+Set Implicit Arguments.
+
+
+
+(* TODO: move to MemoryC *)
+Let Mem_unchanged_on_trans_strong: forall
+      P m0 m1 m2
+      (UNCH0: Mem.unchanged_on P m0 m1)
+      (UNCH1: Mem.unchanged_on (P /2\ (fun b _ => Mem.valid_block m0 b)) m1 m2)
+  ,
+    <<UNCH2: Mem.unchanged_on P m0 m2>>
+.
+Proof. i.
+  inv UNCH0. inv UNCH1.
+  econs; i.
+  - xomega.
+  - etransitivity.
+    { eapply unchanged_on_perm; eauto. }
+    eapply unchanged_on_perm0; eauto.
+    { unfold Mem.valid_block in *. xomega. }
+  - erewrite <- unchanged_on_contents; eauto.
+    dup H0. apply Mem.perm_valid_block in H1. unfold Mem.valid_block in *.
+    erewrite <- unchanged_on_contents0; eauto.
+    eapply unchanged_on_perm; eauto.
+Qed.
+
+
+
+
+
+Record t := mk {
+  unreach:> block -> bool; (* for finiteness' `j` function. *)
+  ge_nb: block;
+  nb: block;
+}
+.
+
+Notation "'prange' '#' hi" := (fun blk => Plt blk hi) (at level 50, no associativity (* , only parsing *)).
+Notation "'prange' lo '#'" := (fun blk => Ple lo blk) (at level 50, no associativity (* , only parsing *)).
+Notation "'prange' lo hi" := (fun blk => Ple lo blk /\ Plt blk hi) (at level 50, no associativity (* , only parsing *)).
+
+Inductive wf (su: t): Prop :=
+| wf_intro
+  (WFLO: su <1= prange su.(ge_nb) #)
+  (WFHI: su <1= prange # su.(nb))
+.
+
+(* One strong point of definiton compared to inductive:
+elimination of multiple predicate requires
+- (inductive) multiple "inv"
+- (definition) unfold __ in *; des *)
+Definition hle_old (su0 su1: t): Prop :=
+  (<<PRIV: su0.(unreach) <1= su1.(unreach)>>)
+  /\
+  (<<OLD: su1.(unreach) /1\ (prange # su0.(nb)) <1= su0.(unreach)>>)
+  /\
+  (<<NB: Ple su0.(nb) su1.(nb)>>)
+  /\
+  (<<GENB: su0.(ge_nb) = su1.(ge_nb)>>)
+.
+
+Definition hle (su0 su1: t): Prop :=
+  (<<OLD: forall blk (LT: Plt blk su0.(nb)), su0 blk = su1 blk>>)
+  /\
+  (<<NB: Ple su0.(nb) su1.(nb)>>)
+  /\
+  (<<GENB: su0.(ge_nb) = su1.(ge_nb)>>)
+.
+
+Lemma hle_old_hle: forall su0 su1, hle_old su0 su1 -> hle su0 su1.
+Proof.
+  split; i; rr in H; des; rr; esplits; eauto.
+  - ii. destruct (su1 blk) eqn:T; ss.
+    + exploit OLD; eauto.
+    + destruct (su0 blk) eqn:T2; ss. exploit PRIV; eauto.
+Qed.
+Lemma hle_hle_old: forall su0 su1 (WF: wf su0), hle su0 su1 -> hle_old su0 su1.
+Proof.
+  split; i; rr in H; des; rr; esplits; eauto.
+  - i. erewrite <- OLD; eauto.
+    inv WF. exploit WFHI; eauto.
+  - i. des. erewrite OLD; eauto.
+Qed.
+
+Lemma hle_update
+      (su0 su1 su2: t)
+      (EQ: forall blk (LT: Plt blk su0.(nb)), su1 blk = su2 blk)
+      (NB: Ple su1.(nb) su2.(nb))
+      (GENB: su1.(ge_nb) = su2.(ge_nb))
+      (HLE: hle su0 su1)
+  :
+    <<HLE: hle su0 su2>>
+.
+Proof.
+  rr in HLE. des.
+  rr. esplits; eauto; try xomega.
+  - rewrite <- GENB. ss.
+Qed.
+
+Lemma hle_old_update
+      (su0 su1 su2: t)
+      (EQ: forall blk (LT: Plt blk su0.(nb)), su1 blk = su2 blk)
+      (NB: Ple su1.(nb) su2.(nb))
+      (GENB: su1.(ge_nb) = su2.(ge_nb))
+      (HLE: hle_old su0 su1)
+      (WF: wf su0)
+  :
+    <<HLE: hle_old su0 su2>>
+.
+Proof.
+  rr in HLE. rr. des. esplits; eauto.
+  - inv WF. i. exploit PRIV; eauto. i. erewrite <- EQ; eauto.
+  - i; des. erewrite <- EQ in PR; eauto.
+  - rewrite <- NB. xomega.
+  - rewrite <- GENB. ss.
+Qed.
+
+Global Program Instance hle_old_PreOrder: PreOrder hle_old.
+Next Obligation.
+  rr. ii; des. esplits; eauto.
+  - ii. des; ss.
+  - xomega.
+Qed.
+Next Obligation.
+  ii; des.
+  unfold hle_old in *. des.
+  esplits; eauto.
+  - ii. des; ss. eapply OLD0; eauto. esplits; eauto. eapply OLD; eauto. esplits; eauto. xomega.
+  - xomega.
+  - congruence.
+Qed.
+
+Global Program Instance hle_PreOrder: PreOrder hle.
+Next Obligation.
+  rr. ii; des. esplits; eauto. reflexivity.
+Qed.
+Next Obligation.
+  ii; des.
+  unfold hle in *. des.
+  esplits; eauto.
+  - ii. rewrite <- OLD; ss; try xomega. rewrite OLD0; ss.
+  - xomega.
+  - congruence.
+Qed.
+
+Inductive mle (su: t) (m0 m1: Memory.mem): Prop :=
+| mle_intro
+    (PERM: forall
+        blk ofs
+        (VALID: m0.(Mem.valid_block) blk)
+      ,
+        m1.(Mem.perm) blk ofs Max <1= m0.(Mem.perm) blk ofs Max)
+    (RO: Mem.unchanged_on m0.(loc_not_writable) m0 m1)
+    (PRIV: Mem.unchanged_on (fun _ => su).(Basics.flip) m0 m1)
+.
+
+Global Program Instance mle_PreOrder su: PreOrder (mle su).
+Next Obligation.
+  rr. ii. econs; eauto with mem.
+Qed.
+Next Obligation.
+  ii. inv H. inv H0. econs; ss; eauto.
+  - ii. eapply PERM; eauto. eapply PERM0; eauto. unfold Mem.valid_block in *. inv RO. xomega.
+  - eapply Mem_unchanged_on_trans_strong; eauto.
+    eapply Mem.unchanged_on_implies; try apply RO0; eauto.
+    ii. des. rr in H. eapply H; eauto.
+  - eapply Mem.unchanged_on_trans; eauto.
+Qed.
+
+Lemma store_mle
+      chunk m0 blk ofs v m1
+      (STR: Mem.store chunk m0 blk ofs v = Some m1)
+      (su: t)
+      (SU: ~su blk)
+  :
+    <<MLE: mle su m0 m1>>
+.
+Proof.
+  econs; eauto.
+  - ii. eauto with mem.
+  - (* Copied from Events.volatile_store_readonly *)
+    eapply Mem.store_unchanged_on; eauto.
+    exploit Mem.store_valid_access_3; eauto. intros [P Q].
+    intros. unfold loc_not_writable. red; intros. elim H0.
+    apply Mem.perm_cur_max. apply P. auto.
+  - eapply Mem.store_unchanged_on; eauto.
+Qed.
+
+Lemma free_mle
+      m0 blk lo hi m1
+      (FREE: Mem.free m0 blk lo hi = Some m1)
+      (su: t)
+      (SU: ~su blk)
+  :
+    <<MLE: mle su m0 m1>>
+.
+Proof.
+  econs; eauto.
+  - ii. eauto with mem.
+  - (* Copied from Events.extcall_free_ok *)
+    inv FREE. eapply Mem.free_unchanged_on; eauto.
+    intros. red; intros. elim H1.
+    apply Mem.perm_cur_max. apply Mem.perm_implies with Freeable; auto with mem.
+    eapply Mem.free_range_perm; eauto.
+  - eapply Mem.free_unchanged_on; eauto.
+Qed.
+
+Lemma storebytes_mle
+      m0 blk ofs mvs m1
+      (STR: Mem.storebytes m0 blk ofs mvs = Some m1)
+      (su: t)
+      (SU: ~su blk)
+  :
+    <<MLE: mle su m0 m1>>
+.
+Proof.
+  econs; eauto.
+  - ii. eauto with mem.
+  - (* Copied from Events.volatile_store_readonly *)
+    inv STR. eapply Mem.storebytes_unchanged_on; eauto.
+    intros. red; intros. elim H1.
+    apply Mem.perm_cur_max.
+    eapply Mem.storebytes_range_perm; eauto.
+  - eapply Mem.storebytes_unchanged_on; eauto.
+Qed.
+
+Lemma alloc_mle
+      m0 lo hi m1 blk
+      (ALC: Mem.alloc m0 lo hi = (m1, blk))
+      (su: t)
+  :
+    <<MLE: mle su m0 m1>>
+.
+Proof.
+  econs; eauto.
+  - ii. eauto with mem.
+  - eapply Mem.alloc_unchanged_on; eauto.
+  - eapply Mem.alloc_unchanged_on; eauto.
+Qed.
+
+Lemma mle_monotone
+      (su0 su1: t)
+      (LE: su0 <1= su1)
+      m0 m1
+      (MLE: su1.(mle) m0 m1)
+  :
+    <<MLE: su0.(mle) m0 m1>>
+.
+Proof.
+  inv MLE. econs; eauto. eapply Mem.unchanged_on_implies; eauto. unfold Basics.flip in *. rr. ii. eapply LE; eauto.
+Qed.
+
+Ltac nb_tac :=
+  repeat
+    multimatch goal with
+    | [ H: nb _ = _ |- _ ] => rewrite H in *
+    | [ H: ge_nb _ = _ |- _ ] => rewrite H in *
+    end
+.
